random export.v changes

CPPSynth/export.v
@@ -5,3 +5,20 @@ Require
 Require Import ExportSExpr.ExportSExpr.
 
 ExportSExpr CPPSynth.SExpression.
+
+Class C1 (T : Set) : Set :=
+{
+  method1 : forall (t : T), bool * T ;
+  method2 : forall (x : nat) (t : T), T
+}.
+
+Inductive acc_state : Set :=
+  | acc_state_make : forall (n : nat), acc_state.
+
+Instance C1A : C1 acc_state :=
+{|
+  method1 := fun (t : acc_state) => match t with | acc_state_make O => (true, t) | _ => (false, t) end ;
+  method2 := fun (x : nat) (t : acc_state) => match t with | acc_state_make y => acc_state_make (x + y) end 
+|}.
+
+ExportSExpr method1.
